# baseURI: http://resource.isamples.org/vocabulary/sampledFeature/ontology
# imports: http://www.w3.org/2004/02/skos/core

@prefix : <http://resource.isamples.org/vocabulary/sampledFeature/> .
@prefix dct: <http://purl.org/dc/terms/> .
@prefix owl: <http://www.w3.org/2002/07/owl#> .
@prefix rdf: <http://www.w3.org/1999/02/22-rdf-syntax-ns#> .
@prefix rdfs: <http://www.w3.org/2000/01/rdf-schema#> .
@prefix sf: <http://resource.isamples.org/vocabulary/sampledFeature/> .
@prefix skos: <http://www.w3.org/2004/02/skos/core#> .
@prefix xsd: <http://www.w3.org/2001/XMLSchema#> .

<http://resource.isamples.org/vocabulary/sampledFeature/ontology>
  rdf:type owl:Ontology ;
  dct:created "2021-03-17"^^xsd:date ;
  dct:creator <https://orcid.org/0000-0001-6041-5302> ;
  dct:license <https://creativecommons.org/licenses/by/4.0/legalcode> ;
  dct:modified "2021-03-17"^^xsd:date ;
  owl:imports <http://www.w3.org/2004/02/skos/core> ;
  owl:versionInfo "0.1" ;
.

<https://orcid.org/0000-0001-6041-5302>
  rdf:type owl:NamedIndividual ;
  rdfs:comment "e-mail: mailto:smrTucson@gmail.com " ;
  rdfs:comment "orchid-id: https://orcid.org/0000-0001-6041-5302" ;
  rdfs:label "Dr. Stephen M. Richard" ;
.

sf:aggregationspecimen
  rdf:type skos:Concept ;
  rdfs:label "aggregation specimen"@en ;
  skos:broader sf:existingspecimen ;
  skos:definition "specimen is derived by processing of an aggregation material parent specimen"@en ;
  skos:inScheme sf:vocabulary ;
  skos:prefLabel "aggregation specimen"@en ;
.
sf:animalorganism
  rdf:type skos:Concept ;
  rdfs:label "animal organism"@en ;
  skos:broader sf:biologicalorganism ;   skos:inScheme sf:vocabulary ;
  skos:definition "specimen samples a living animal organism" ;
  skos:prefLabel "animal organism"@en ;
.
sf:anysampledfeature
  rdf:type skos:Concept ;
  rdfs:label "any sampled feature "@en ;
  skos:prefLabel "any sampled feature "@en ;  
  skos:topConceptOf sf:vocabulary ;
.
sf:aquifer
  rdf:type skos:Concept ;
  rdfs:label "aquifer"@en ;
  skos:broader sf:formationliquid ;
  skos:definition "Specimen samples water that resides in fractures or intergranular porosity in the solid earth."@en ;   skos:inScheme sf:vocabulary ;
  skos:prefLabel "aquifer"@en ;
.
sf:atmosphere
  rdf:type skos:Concept ;
  rdfs:label "atmosphere"@en ;
  skos:broader sf:earthenvironment ;   skos:inScheme sf:vocabulary ;
  skos:definition "specimen samples the earth atmosphere"@en ;
  skos:prefLabel "atmosphere"@en ;
.
sf:biologicalorganism
  rdf:type skos:Concept ;
  rdfs:label "Biological organism"@en ;
  skos:broader sf:anysampledfeature ;   skos:inScheme sf:vocabulary ;
  skos:definition "specimen samples a living organism"@en ;
  skos:prefLabel "Biological organism"@en ;
.
sf:building
  rdf:type skos:Concept ;
  rdfs:label "Building"@en ;
  skos:broader sf:humanoccupationsite ;   skos:inScheme sf:vocabulary ;
  skos:definition "specimen samples materials or objects related to human structures"@en ;
  skos:prefLabel "Building"@en ;
.
sf:earthenvironment
  rdf:type skos:Concept ;
  rdfs:label "Earth environment"@en ;
  skos:broader sf:anysampledfeature ;   skos:inScheme sf:vocabulary ;
  skos:definition "specimen samples the natural earth environment"@en ;
  skos:prefLabel "Earth environment"@en ;
.
sf:earthsurface
  rdf:type skos:Concept ;
  rdfs:label "Earth Surface"@en ;
  skos:broader sf:earthenvironment ;   skos:inScheme sf:vocabulary ;
  skos:definition "Specimen samples the interface between solid earth, hydrosphere, or atmosphere" ;
  skos:prefLabel "Earth Surface"@en ;
.
sf:existingspecimen
  rdf:type skos:Concept ;
  rdfs:label "Existing specimen"@en ;
  skos:broader sf:anysampledfeature ;   skos:inScheme sf:vocabulary ;
  skos:definition "specimen is derived by processing of a parent specimen"@en ;
  skos:inScheme sf:vocabulary ;
  skos:prefLabel "Existing specimen"@en ;
.
sf:extraterrestrialenvironment
  rdf:type skos:Concept ;
  rdfs:label "extraterrestrial environment "@en ;
  skos:broader sf:anysampledfeature ;
  skos:definition "specimen samples environment outside of solid earth, hydrosphere, or atmosphere."@en ;   skos:inScheme sf:vocabulary ;
  skos:prefLabel "extraterrestrial environment "@en ;
.
sf:flowingwater
  rdf:type skos:Concept ;
  rdfs:label "Flowing water"@en ;
  skos:broader sf:terrrestrialwaterbody ;
  skos:definition "specimen samples  a flowing water body (river, stream..)"@en ;
  skos:prefLabel "Flowing water"@en ;   skos:inScheme sf:vocabulary ;
.
sf:fluidspecimen
  rdf:type skos:Concept ;
  rdfs:label "fluid specimen "@en ;
  skos:broader sf:existingspecimen ;
  skos:definition "specimen is derived by processing of a fluid (liquid or gas) material parent specimen"@en ;   skos:inScheme sf:vocabulary ;
  skos:prefLabel "fluid specimen "@en ;
.
sf:forestfloor
  rdf:type skos:Concept ;
  rdfs:label "forest floor"@en ;   skos:inScheme sf:vocabulary ;
  skos:broader sf:earthsurface ;
  skos:definition "Specimen samples a forest floor interface with the atmosphere" ;
  skos:prefLabel "forest floor"@en ;
.
sf:formationgas
  rdf:type skos:Concept ;
  rdfs:label "formation gas"@en ;
  skos:broader sf:subsurfacefluidreservoir ;   skos:inScheme sf:vocabulary ;
  skos:definition "Specimen samples gaseous material that resides in fractures or intergranular porosity in the solid earth."@en ;
  skos:prefLabel "formation gas"@en ;
.
sf:formationliquid
  rdf:type skos:Concept ;
  rdfs:label "formation liquid"@en ;
  skos:broader sf:subsurfacefluidreservoir ;   skos:inScheme sf:vocabulary ;
  skos:definition "Specimen samples liquid that resides in fractures or intergranular porosity in the solid earth."@en ;
  skos:prefLabel "formation liquid"@en ;
.
sf:gasspecimen
  rdf:type skos:Concept ;
  rdfs:label "gas specimen"@en ;   skos:inScheme sf:vocabulary ;
  skos:broader sf:fluidspecimen ;
  skos:definition "specimen is derived by processing of a gaseous  parent specimen"@en ;
  skos:prefLabel "gas specimen "@en ;
.
sf:humanoccupationsite
  rdf:type skos:Concept ;
  rdfs:label "Human occupation site "@en ;
  skos:broader sf:anysampledfeature ;   skos:inScheme sf:vocabulary ;
  skos:definition "specimen samples materials or objects produced by human activity"@en ;
  skos:prefLabel "Human occupation site "@en ;
.
sf:labenvironment
  rdf:type skos:Concept ;
  rdfs:label "lab environment"@en ;   skos:inScheme sf:vocabulary ;
  skos:definition "specimen samples the environment in a laboratory" ;
  skos:prefLabel "lab environment"@en ;
.
sf:laboratoryenvironment
  rdf:type skos:Concept ;
  rdfs:label "Laboratory environment"@en ;   skos:inScheme sf:vocabulary ;
  skos:broader sf:anysampledfeature ;
  skos:definition "specimen samples environment in a laboratory"@en ;
  skos:prefLabel "Laboratory environment "@en ;
.
sf:lake
  rdf:type skos:Concept ;
  rdfs:label "Lake"@en ;   skos:inScheme sf:vocabulary ;
  skos:broader sf:terrrestrialwaterbody ;
  skos:definition "specimen samples  a relatively static water body (lake)"@en ;
  skos:prefLabel "Lake"@en ;
.
sf:liquidspecimen
  rdf:type skos:Concept ;
  rdfs:label "liquid specimen "@en ;   skos:inScheme sf:vocabulary ;
  skos:broader sf:fluidspecimen ;
  skos:definition "specimen is derived by processing of a liquid  parent specimen"@en ;
  skos:prefLabel "liquid specimen "@en ;
.
sf:marineenvironment
  rdf:type skos:Concept ;
  rdfs:label "Marine environment"@en ;
  skos:broader sf:waterbody ;   skos:inScheme sf:vocabulary ;
  skos:definition "specimen samples marine hydrosphere"@en ;
  skos:prefLabel "Marine environment"@en ;
.
sf:microbialorganism
  rdf:type skos:Concept ;
  rdfs:label "microbial organism"@en ;   skos:inScheme sf:vocabulary ;
  skos:broader sf:biologicalorganism ;
  skos:definition "specimen samples a living microorganism"@en ;
  skos:prefLabel "microbial organism"@en ;
.
sf:mineralspecies
  rdf:type skos:Concept ;
  rdfs:label "mineral species"@en ;   skos:inScheme sf:vocabulary ;
  skos:broader sf:solidearth ;
  skos:definition "Specimen samples a particular mineral species" ;
  skos:prefLabel "mineral species"@en ;
.
sf:plantfoliage
  rdf:type skos:Concept ;
  rdfs:label "plant foliage"@en ;   skos:inScheme sf:vocabulary ;
  skos:broader sf:plantorganism ;
  skos:definition "specimen samples leaves from a plat organism"@en ;
  skos:prefLabel "plant foliage"@en ;
.
sf:plantorganism
  rdf:type skos:Concept ;
  rdfs:label "plant organism"@en ;
  skos:broader sf:biologicalorganism ;   skos:inScheme sf:vocabulary ;
  skos:definition "specimen samples a living plant organism"@en ;
  skos:prefLabel "plant organism"@en ;
.
sf:regolithlayer
  rdf:type skos:Concept ;
  rdfs:label "Regolith layer"@en ;
  skos:broader sf:solidearth ;   skos:inScheme sf:vocabulary ;
  skos:definition "Specimen samples material formed at the interface between the solid earth and atmosphere, but not at the surface. Soil, regolith" ;
  skos:prefLabel "Regolith layer"@en ;
.
sf:riverorstreambed
  rdf:type skos:Concept ;
  rdfs:label "River or stream bed"@en ;
  skos:broader sf:waterbodybottom ;   skos:inScheme sf:vocabulary ;
  skos:definition "Specimen samples the solid earth  interface a flowing water body"@en ;
  skos:prefLabel "River or stream bed"@en ;
.
sf:rocksample
  rdf:type skos:Concept ;
  rdfs:label "Rock sample"@en ;   skos:inScheme sf:vocabulary ;
  skos:definition "specimen is derived by processing of a solid rock object parent specimen" ;
  skos:prefLabel "Rock sample"@en ;
.
sf:rocksubsample
  rdf:type skos:Concept ;
  rdfs:label "rock subsample"@en ;
  skos:broader sf:solidspecimen ;   skos:inScheme sf:vocabulary ;
  skos:definition "specimen is derived by processing of a solid rock object parent specimen"@en ;
  skos:prefLabel "rock subsample"@en ;
.
sf:section
  rdf:type skos:Concept ;
  rdfs:label "Section"@en ;
  skos:broader sf:solidearth ;   skos:inScheme sf:vocabulary ;
  skos:definition "Specimen samples a vertical transect within the solid earth"@en ;
  skos:prefLabel "Section"@en ;
.
sf:solidearth
  rdf:type skos:Concept ;
  rdfs:label "Solid Earth"@en ;
  skos:broader sf:earthenvironment ;   skos:inScheme sf:vocabulary ;
  skos:definition "Specimen samples the solid earth" ;
  skos:prefLabel "Solid Earth"@en ;
.
sf:solidspecimen
  rdf:type skos:Concept ;
  rdfs:label "solid specimen "@en ;
  skos:broader sf:existingspecimen ;   skos:inScheme sf:vocabulary ;
  skos:definition "specimen is derived by processing of a solid object parent specimen"@en ;
  skos:prefLabel "solid specimen "@en ;
.
sf:stephen_richard
  rdf:type owl:NamedIndividual ;
  rdfs:comment "e-mail: mailto:smrTucson@gmail.com " ;
  rdfs:comment "orchid-id: https://orcid.org/0000-0001-6041-5302" ;
  rdfs:label "Dr. Stephen M. Richard" ;
.
sf:subsurfacefluidreservoir
  rdf:type skos:Concept ;
  rdfs:label "Subsurface fluid reservoir"@en ;
  skos:broader sf:earthenvironment ;   skos:inScheme sf:vocabulary ;
  skos:definition "Specimen samples fluid that resides in fractures or intergranular porosity in the solid earth."@en ;
  skos:prefLabel "Subsurface fluid reservoir"@en ;
.
sf:terrestrialsection
  rdf:type skos:Concept ;
  rdfs:label "terrestrial section"@en ;   skos:inScheme sf:vocabulary ;
  skos:broader sf:section ;
  skos:definition "Specimen samples a vertical transect within the solid earth, not beneath a marine water body"@en ;
  skos:prefLabel "terrestrial section"@en ;
.
sf:terrrestrialwaterbody
  rdf:type skos:Concept ;
  rdfs:label "terrrestrial water body"@en ;   skos:inScheme sf:vocabulary ;
  skos:broader sf:waterbody ;
  skos:definition "specimen samples terrestrial hydrosphere-- lake, other standing water, or a flowing water body (river, stream..)"@en ;
  skos:prefLabel "terrrestrial water body"@en ;
.
sf:vocabulary
  rdf:type skos:ConceptScheme ;
  rdfs:label "Sampled Feature vocabulary"@en ;
  skos:prefLabel "Sampled Feature vocabulary"@en ;
.
sf:waterbody
  rdf:type skos:Concept ;
  rdfs:label "Water body"@en ;
  skos:broader sf:earthenvironment ;   skos:inScheme sf:vocabulary ;
  skos:definition "specimen samples the hydrosphere"@en ;
  skos:prefLabel "Water body"@en ;
.
sf:waterbodybottom
  rdf:type skos:Concept ;
  rdfs:label "water body bottom"@en ;   skos:inScheme sf:vocabulary ;
  skos:broader sf:earthsurface ;
  skos:broader sf:waterbody ;
  skos:definition "Specimen samples the solid earth  interface with the hydrosphere"@en ;
  skos:prefLabel "water body bottom"@en ;
.
sf:waterbodysurface
  rdf:type skos:Concept ;
  rdfs:label "water body surface"@en ;   skos:inScheme sf:vocabulary ;
  skos:broader sf:earthsurface ;
  skos:broader sf:waterbody ;
  skos:definition "Specimen samples the  interface between hydrosphere and atmosphere"@en ;
  skos:prefLabel "water body surface"@en ;
.
