# baseURI: http://resource.isamples.org/vocabulary/specimentype/ontology
# imports: http://www.w3.org/2004/02/skos/core

@prefix : <http://resource.isamples.org/vocabulary/specimentype/> .
@prefix dct: <http://purl.org/dc/terms/> .
@prefix owl: <http://www.w3.org/2002/07/owl#> .
@prefix rdf: <http://www.w3.org/1999/02/22-rdf-syntax-ns#> .
@prefix rdfs: <http://www.w3.org/2000/01/rdf-schema#> .
@prefix skos: <http://www.w3.org/2004/02/skos/core#> .
@prefix spt: <http://resource.isamples.org/vocabulary/specimentype/> .
@prefix xsd: <http://www.w3.org/2001/XMLSchema#> .

spt:aggregation
  rdf:type skos:Concept ;
  rdfs:comment "Sample consists of a bunch of material fragments, not related to the same object (e.g. not a bunch of broken pot sherds that might be reassembled), but taken together representative of the sampled feature. Examples: loose soil, sediment, crushed rock,  particulate, including (non-biological) filtrates and residues. The sample requires some kind of container to keep it together. Cores of loosely consolidated material are considered 'piece of solid material' because the internal parts have spatial relationships (e.g. upper part, lower part)."@en ;
  rdfs:label "Aggregation specimen "@en ;
  skos:broader spt:physicalspecimen ;
  skos:prefLabel "Aggregation specimen "@en ;
.
spt:artifact
  rdf:type skos:Concept ;
  rdfs:comment "An object made (manufactured, shaped, modified) by a human being, or precursor hominid. Include a set of pieces belonging originally to a single object and treated as a single specimen."@en ;
  rdfs:label "Artifact "@en ;
  skos:broader spt:piecesolidmaterial ;
  skos:inScheme spt:specimenttypevocabulary ;
  skos:prefLabel "Artifact "@en ;
.
spt:biologicalspecimen
  rdf:type skos:Concept ;
  rdfs:comment "Specimen for which the sampled feature is one or more living organisms from a particular biome context, megascopic or microscopic"@en ;
  rdfs:label "Biological specimen"@en ;
  skos:broader spt:physicalspecimen ;
  skos:inScheme spt:specimenttypevocabulary ;
  skos:prefLabel "Biological specimen"@en ;
.
spt:biomeaggregation
  rdf:type skos:Concept ;
  rdfs:comment "Specimen is an aggregation of whole or fragmentary parts of multiple organisms representative of some site."@en ;
  rdfs:label "Biome aggregation specimen "@en ;
  skos:broader spt:aggregation ;
  skos:broader spt:biologicalspecimen ;
  skos:inScheme spt:specimenttypevocabulary ;
  skos:prefLabel "Biome aggregation specimen "@en ;
.
spt:containerfluid
  rdf:type skos:Concept ;
  rdfs:comment "Liquid, gas, or mixed dominantly fluid phases in a container.  Includes colloids, foams, gels, suspensions. The sampled feature is the fluid substance; fluid samples collected to analyze the contained biome should be considered *Biome Aggregation*"@en ;
  rdfs:label "Container with fluid "@en ;
  skos:broader spt:physicalspecimen ;
  skos:inScheme spt:specimenttypevocabulary ;
  skos:prefLabel "Container with fluid "@en ;
.
spt:fossil
  rdf:type skos:Concept ;
  rdfs:comment "Specimen is fossilized remains of one or more organism preserved in rock; includes whole body, body parts (usually bone or shell), and trace fossils."@en ;
  rdfs:label "Fossil "@en ;
  skos:broader spt:piecesolidmaterial ;
  skos:inScheme spt:specimenttypevocabulary ;
  skos:prefLabel "Fossil "@en ;
.
spt:ontology
  rdf:type owl:Ontology ;
  dct:created "2021-03-24"^^xsd:date ;
  dct:creator <https://orcid.org/0000-0001-6041-5302> ;
  dct:license <https://creativecommons.org/licenses/by/4.0/legalcode> ;
  dct:modified "2021-03-24"^^xsd:date ;
  owl:imports <http://www.w3.org/2004/02/skos/core> ;
  owl:versionInfo "0.1" ;
.
spt:organismpart
  rdf:type skos:Concept ;
  rdfs:comment "Part of an organism, e.g. a tissue sample, plant leaf, flower, bird feather, bone, shell or other hard body part (not fossilized).  Does not necessarily imply existance of parent sample. Not fossilized; generally includes organism parts native to deposits of Holocene to Recent age."@en ;
  rdfs:label "Organism part "@en ;
  skos:broader spt:biologicalspecimen ;
  skos:broader spt:specimenpart ;
  skos:inScheme spt:specimenttypevocabulary ;
  skos:prefLabel "Organism part "@en ;
.
spt:physicalspecimen
  rdf:type skos:Concept ;
  rdfs:comment "top concept in specimen type hierarchy. Represents any physical specimen."@en ;
  rdfs:label "Physical specimen"@en ;
  skos:prefLabel "Physical specimen"@en ;
  skos:topConceptOf spt:specimenttypevocabulary ;
.
spt:piecesolidmaterial
  rdf:type skos:Concept ;
  rdfs:comment "Single piece of material not one of the other types, e.g. rock specimen, mineral specimen, core. Ice and permafrost are considered solid materials. Includes set of pieces belonging originally to a single object and treated as a single specimen."@en ;
  rdfs:label "Piece of Solid Material "@en ;
  skos:broader spt:physicalspecimen ;
  skos:inScheme spt:specimenttypevocabulary ;
  skos:prefLabel "Piece of Solid Material "@en ;
.
spt:specimenpart
  rdf:type skos:Concept ;
  rdfs:comment "" ;
  rdfs:label "Specimen part "@en ;
  skos:broader spt:physicalspecimen ;
  skos:inScheme spt:specimenttypevocabulary ;
  skos:prefLabel "Specimen part "@en ;
.
spt:specimenttypevocabulary
  rdf:type skos:ConceptScheme ;
  rdfs:comment "Broad categories to classify any kind of physical specimen"@en ;
  rdfs:label "iSamples Specimen Type Vocabulary "@en ;
  skos:prefLabel "iSamples Specimen Type Vocabulary "@en ;
.
spt:wholeorganism
  rdf:type skos:Concept ;
  rdfs:comment "Specimen consists of the bodies of one or more entire organisms of the same species, from any kingdom."@en ;
  rdfs:label "Whole organism specimen "@en ;
  skos:broader spt:biologicalspecimen ;
  skos:inScheme spt:specimenttypevocabulary ;
  skos:prefLabel "Whole organism specimen "@en ;
.
<https://orcid.org/0000-0001-6041-5302>
  rdf:type owl:NamedIndividual ;
  rdfs:comment "e-mail: mailto:smrTucson@gmail.com " ;
  rdfs:comment "orchid-id: https://orcid.org/0000-0001-6041-5302" ;
  rdfs:label "Dr. Stephen M. Richard" ;
.
