# baseURI: http://resource.isamples.org/vocabulary/specimentype/ontology
# imports: http://www.w3.org/2004/02/skos/core

@prefix : <http://resource.isamples.org/vocabulary/specimentype/> .
@prefix dct: <http://purl.org/dc/terms/> .
@prefix owl: <http://www.w3.org/2002/07/owl#> .
@prefix rdf: <http://www.w3.org/1999/02/22-rdf-syntax-ns#> .
@prefix spt: <http://resource.isamples.org/vocabulary/specimentype/> .
@prefix xml: <http://www.w3.org/XML/1998/namespace> .
@prefix xsd: <http://www.w3.org/2001/XMLSchema#> .
@prefix rdfs: <http://www.w3.org/2000/01/rdf-schema#> .
@prefix skos: <http://www.w3.org/2004/02/skos/core#> .
@base <http://resource.isamples.org/vocabulary/specimentype/ontology> .

<http://resource.isamples.org/vocabulary/specimentype/ontology> rdf:type owl:Ontology ;
                                                                 owl:imports <http://www.w3.org/2004/02/skos/core> ;
                                                                 dct:created "2021-03-24"^^xsd:date ;
                                                                 dct:creator <https://orcid.org/0000-0001-6041-5302> ;
                                                                 dct:license <https://creativecommons.org/licenses/by/4.0/legalcode> ;
                                                                 dct:modified "2021-03-24"^^xsd:date .

#################################################################
#    Annotation properties
#################################################################

###  http://purl.org/dc/terms/created
dct:created rdf:type owl:AnnotationProperty .


###  http://purl.org/dc/terms/license
dct:license rdf:type owl:AnnotationProperty .


###  http://purl.org/dc/terms/modified
dct:modified rdf:type owl:AnnotationProperty .


#################################################################
#    Individuals
#################################################################

###  http://resource.isamples.org/vocabulary/specimentype/analyticalpreparation
spt:analyticalpreparation rdf:type owl:NamedIndividual ,
                                   skos:Concept ;
                          skos:broader spt:researchproduct ;
                          rdfs:comment "e.g. thin section, XRF bead, SEM stub, rock powder. If identified separately, this should have a ‘parent’ link to the original sample"@en ;
                          rdfs:label "Analytical preparation "@en ;
                          skos:prefLabel "Analytical preparation  "@en .


###  http://resource.isamples.org/vocabulary/specimentype/anthropogenicaggregation
spt:anthropogenicaggregation rdf:type owl:NamedIndividual ,
                                      skos:Concept ;
                             skos:broader spt:anyaggregation ;
                             skos:inScheme spt:specimenttypevocabulary ;
                             rdfs:label "Anthropogenic aggregation"@en ;
                             skos:definition "Aggregation consists of fragments of material produced by human activity,  not described individually, and generally not all originating from the same object.  Includes pottery in an excavation unit [that] gets an aggregate description, production waste, production raw-materials, or other residues (broken bits of plaster from an destroyed wall), synthetic powders."@en ;
                             skos:prefLabel "Anthropogenic aggregation"@en .


###  http://resource.isamples.org/vocabulary/specimentype/anyaggregation
spt:anyaggregation rdf:type owl:NamedIndividual ,
                            skos:Concept ;
                   skos:broader spt:physicalspecimen ;
                   rdfs:comment "Sample consists of a bunch of material fragments, not related to the same object (e.g. not a bunch of broken pot sherds that might be reassembled), but taken together representative of the sampled feature. Examples: loose soil, sediment, crushed rock,  particulate, bunches of unrelated pot sherd, human production waste, filtrates and residues. The sample requires some kind of container to keep it together. Cores of loosely consolidated material are considered 'piece of solid material' because the internal parts have spatial relationships (e.g. upper part, lower part)."@en ;
                   rdfs:label "Any aggregation specimen"@en ;
                   skos:prefLabel "Any aggregation specimen"@en .


###  http://resource.isamples.org/vocabulary/specimentype/artifact
spt:artifact rdf:type owl:NamedIndividual ,
                      skos:Concept ;
             skos:broader spt:physicalspecimen ;
             skos:inScheme spt:specimenttypevocabulary ;
             rdfs:comment "An object made (manufactured, shaped, modified) by a human being, or precursor hominid. Include a set of pieces belonging originally to a single object and treated as a single specimen."@en ;
             rdfs:label "Artifact "@en ;
             skos:prefLabel "Artifact "@en .


###  http://resource.isamples.org/vocabulary/specimentype/biologicalspecimen
spt:biologicalspecimen rdf:type owl:NamedIndividual ,
                                skos:Concept ;
                       skos:broader spt:physicalspecimen ;
                       skos:inScheme spt:specimenttypevocabulary ;
                       rdfs:comment "Specimen for which the sampled feature is one or more living organisms from a particular biome context, megascopic or microscopic"@en ;
                       rdfs:label "Any biological specimen"@en ;
                       skos:prefLabel "Any biological specimen"@en .


###  http://resource.isamples.org/vocabulary/specimentype/biomeaggregation
spt:biomeaggregation rdf:type owl:NamedIndividual ,
                              skos:Concept ;
                     skos:broader spt:anyaggregation ,
                                  spt:biologicalspecimen ;
                     skos:inScheme spt:specimenttypevocabulary ;
                     rdfs:comment "Specimen is an aggregation of whole or fragmentary parts of multiple organisms, microscopic or megascopic, representative of some site."@en ;
                     rdfs:label "Biome aggregation specimen "@en ;
                     skos:prefLabel "Biome aggregation specimen "@en .


###  http://resource.isamples.org/vocabulary/specimentype/experimentalproduct
spt:experimentalproduct rdf:type owl:NamedIndividual ,
                                 skos:Concept ;
                        skos:broader spt:researchproduct ;
                        rdfs:comment "Specimen is product of an experimental procedure (e.g. synthetic material)"@en ;
                        rdfs:label "Experiment product "@en ;
                        skos:prefLabel "Experiment product  "@en .


###  http://resource.isamples.org/vocabulary/specimentype/fossil
spt:fossil rdf:type owl:NamedIndividual ,
                    skos:Concept ;
           skos:broader spt:physicalspecimen ;
           skos:inScheme spt:specimenttypevocabulary ;
           rdfs:comment "Specimen is the remains of one or more organisms preserved in rock; includes whole body, body parts (usually bone or shell), and trace fossils. An organism or organism part becomes a fossil when it has undergone some fossilization process that generally entails physical and chemical changes akin to diagenesis in a sedimentary rock. Trace fossils are manifestations of biologic activity preserved in a rock body (typically sedimentary), without included preserved body parts."@en ;
           rdfs:label "Fossil "@en ;
           skos:note "There are many processes that lead to fossilization, including permineralization, casts and molds, authigenic mineralization, replacement and recrystallization, adpression, carbonization, and bioimmuration (https://en.wikipedia.org/wiki/Fossil)."@en ;
           skos:prefLabel "Fossil "@en .


###  http://resource.isamples.org/vocabulary/specimentype/genericaggregation
spt:genericaggregation rdf:type owl:NamedIndividual ,
                                skos:Concept ;
                       skos:broader spt:anyaggregation ;
                       rdfs:label "Aggregation"@en ;
                       skos:definition "An aggregate specimen that is not biogenic or anthropogenic.  Examples: borehole cuttings, loose soil or sediment (e.g. in a bag), rock chips, particulate filtrate or precipitate; rock powders."@en ;
                       skos:prefLabel "Aggregation"@en .


###  http://resource.isamples.org/vocabulary/specimentype/liquidorgas
spt:liquidorgas rdf:type owl:NamedIndividual ,
                         skos:Concept ;
                skos:broader spt:physicalspecimen ;
                skos:inScheme spt:specimenttypevocabulary ;
                rdfs:comment "Liquid, gas, or mixed dominantly fluid phases, necessarily in some kind of container to maintain identity. Might include minor solid particles. Container typically human made, but also includes natural fluid container, e.g. fluid inclusion in a mineral grain.  Includes colloids, foams, gels, suspensions. The sampled feature is the fluid substance; fluid samples collected to analyze the contained biome should be considered *Biome Aggregation*"@en ;
                rdfs:label "Liquid or gas"@en ;
                skos:prefLabel "Liquid or gas"@en .


###  http://resource.isamples.org/vocabulary/specimentype/organismpart
spt:organismpart rdf:type owl:NamedIndividual ,
                          skos:Concept ;
                 skos:broader spt:biologicalspecimen ;
                 skos:inScheme spt:specimenttypevocabulary ;
                 rdfs:comment "Part of an organism, e.g. a tissue sample, plant leaf, flower, bird feather. Include internal parts not composed of organic material (e.g. teeth, bone), and hard body parts that are not shed (hoof, horn, tusk, claw).  Hair is tricky, include here for now.  Does not necessarily imply existance of parent sample. Not fossilized; generally includes organism parts native to deposits of Holocene to Recent age."@en ;
                 rdfs:label "Organism part "@en ;
                 skos:prefLabel "Organism part "@en .


###  http://resource.isamples.org/vocabulary/specimentype/organismproduct
spt:organismproduct rdf:type owl:NamedIndividual ,
                             skos:Concept ;
                    skos:broader spt:biologicalspecimen ;
                    skos:inScheme spt:specimenttypevocabulary ;
                    rdfs:comment "Specimen is a thing produced by some organism, generally not composed of organic material or including biological tissue, e.g. Shell, antler, egg shell, coral skeleton (organic tissue not included), fecal matter, cocoon, web.  Consider internal parts not composed of organic material (e.g. teeth, bone) and hard body parts that are not shed (hoof, horn, tusk) to be organism parts."@en ;
                    rdfs:label "Organism product"@en ;
                    skos:prefLabel "Organism product"@en .


###  http://resource.isamples.org/vocabulary/specimentype/othersolidobject
spt:othersolidobject rdf:type owl:NamedIndividual ,
                              skos:Concept ;
                     skos:broader spt:physicalspecimen ;
                     skos:inScheme spt:specimenttypevocabulary ;
                     rdfs:comment "Single piece of material not one of the other types, e.g. rock specimen, mineral specimen, core. Ice and permafrost are considered solid materials."@en ;
                     rdfs:label "Other solid object"@en ;
                     skos:prefLabel "Other solid object"@en .


###  http://resource.isamples.org/vocabulary/specimentype/physicalspecimen
spt:physicalspecimen rdf:type owl:NamedIndividual ,
                              skos:Concept ;
                     skos:topConceptOf spt:specimenttypevocabulary ;
                     rdfs:comment "top concept in specimen type hierarchy.  Represents any physical specimen."@en ;
                     rdfs:label "Physical specimen"@en ;
                     skos:prefLabel "Physical specimen"@en .


###  http://resource.isamples.org/vocabulary/specimentype/researchproduct
spt:researchproduct rdf:type owl:NamedIndividual ,
                             skos:Concept ;
                    skos:broader spt:physicalspecimen ;
                    rdfs:comment "Specimen is a product of some research workflow, e.g. a thin section, an XRF pellet, a grain mount, SEM stub, synthetic rock or mineral ...  In general there should be a link to a parent specimen from which this was derived.  Might be aggregation (e.g. a synthetic material powder) or a solid object."@en ;
                    rdfs:label "Research product"@en ;
                    skos:prefLabel "Research product"@en .


###  http://resource.isamples.org/vocabulary/specimentype/specimenttypevocabulary
spt:specimenttypevocabulary rdf:type owl:NamedIndividual ,
                                     skos:ConceptScheme ;
                            rdfs:comment "Broad categories to classify any kind of physical specimen"@en ;
                            rdfs:label "iSamples Specimen Type Vocabulary "@en ;
                            skos:prefLabel "iSamples Specimen Type Vocabulary "@en .


###  http://resource.isamples.org/vocabulary/specimentype/wholeorganism
spt:wholeorganism rdf:type owl:NamedIndividual ,
                           skos:Concept ;
                  skos:broader spt:biologicalspecimen ;
                  skos:inScheme spt:specimenttypevocabulary ;
                  rdfs:comment "Specimen consists of the bodies of one or more entire organisms of the same species, from any kingdom. Note that are also 'solid object’"@en ;
                  rdfs:label "Whole organism specimen "@en ;
                  skos:prefLabel "Whole organism specimen "@en .


###  https://orcid.org/0000-0001-6041-5302
<https://orcid.org/0000-0001-6041-5302> rdf:type owl:NamedIndividual ;
                                        rdfs:comment "e-mail: mailto:smrTucson@gmail.com " ,
                                                     "orchid-id: https://orcid.org/0000-0001-6041-5302" ;
                                        rdfs:label "Dr. Stephen M. Richard" .


###  Generated by the OWL API (version 4.5.9.2019-02-01T07:24:44Z) https://github.com/owlcs/owlapi
