# baseURI: https://w3id.org/isample/vocabulary/mingroup/0.9/mineralgroupvocabulary
# imports: http://www.w3.org/2004/02/skos/core

@prefix : <https://w3id.org/isample/vocabulary/mingroup/0.9/> .
@prefix dct: <http://purl.org/dc/terms/> .
@prefix ming: <https://w3id.org/isample/vocabulary/mingroup/0.9/> .
@prefix mat: <https://w3id.org/isample/vocabulary/material/0.9/> .
@prefix owl: <http://www.w3.org/2002/07/owl#> .
@prefix rdf: <http://www.w3.org/1999/02/22-rdf-syntax-ns#> .
@prefix rdfs: <http://www.w3.org/2000/01/rdf-schema#> .
@prefix skos: <http://www.w3.org/2004/02/skos/core#> .
@prefix xml: <http://www.w3.org/XML/1998/namespace> .
@prefix xsd: <http://www.w3.org/2001/XMLSchema#> .

dct:created
  rdf:type owl:AnnotationProperty ;
.
dct:license
  rdf:type owl:AnnotationProperty ;
.
dct:modified
  rdf:type owl:AnnotationProperty ;
.
<https://orcid.org/0000-0001-6041-5302>
  rdf:type owl:NamedIndividual ;
  rdfs:comment "e-mail: mailto:smrTucson@gmail.com " ;
  rdfs:comment "orchid-id: https://orcid.org/0000-0001-6041-5302" ;
  rdfs:label "Dr. Stephen M. Richard" ;
.

ming:mineralgroupvocabulary
  rdf:type owl:NamedIndividual ;
  rdf:type owl:Ontology ;
  rdf:type skos:ConceptScheme ;
  dct:created "2022-08-27"^^xsd:date ;
  dct:creator <https://orcid.org/0000-0001-6041-5302> ;
  dct:license <https://creativecommons.org/licenses/by/4.0/legalcode> ;
  dct:modified "2022-08-27"^^xsd:date ;
  rdfs:label "iSamples Mineral Group Vocabulary"@en ;
  owl:imports <http://www.w3.org/2004/02/skos/core> ;
  skos:definition "Vocabulary to extent the mineral material type category with the top level mineral group categories. Uses the Nickel–Strunz mineral classes, which divide minerals into ten classes according to chemical composition and crystal structure. Nickel-Strunz group 10 is not included because that material would be mat:organiccompounds. Version 10 of the classification is modified from v 9 (Strunz and Nickel,2002) by Jim Ferraiolo and others, and now extended and maintained by mindat.org. Some scope notes from linked.data.gov.au. "@en ;
  skos:prefLabel "iSamples Mineral Group Vocabulary "@en ;
  rdf:seeAlso "https://www.webmineral.com/help/StrunzClass.shtml";
  rdf:seeAlso  "https://www.mindat.org/strunz.php" ;
  dct:source "MINERALOGICAL TABLES: by Hugo Strunz and Ernest H. Nickel. E. Schweizerbart’sche Verlagsbuchhandlung, 2002, Stuttgart, Germany (9th edition). 870 p. ISBN number 3-510-65188-X."
.

ming:nativeelementmineral
  rdf:type owl:NamedIndividual ;
  rdf:type skos:Concept ;
  rdfs:label "Mineral-Native Element"@en ;
  skos:broader mat:mineral ;
  skos:definition "Elements that occur in nature in uncombined form with a distinct mineral structure. Includes metals and intermetallic alloys; metalloids and nonmetals; carbides, silicides, nitrides, phosphides"@en ;
  skos:exactMatch <http://linked.data.gov.au/def/minerals/elements-metals-and-intermetallic-alloys-metalloids-and-nonmetals-carbides-silicides-nitrides-phosphides> ;
  skos:inScheme ming:mineralgroupvocabulary ;
  skos:prefLabel "Mineral-Native Element"@en ;
  skos:altLabel "Nickel-Strunz class 01"@en ;
  rdf:seeAlso "https://www.mindat.org/strunz.php?a=1" ;
.
ming:sulfidesulfosaltmineral
  rdf:type owl:NamedIndividual ;
  rdf:type skos:Concept ;
  rdfs:label "Mineral-Sulfide or Sulfosalt"@en ;
  skos:broader mat:mineral ;
  skos:definition "Sulfide minerals are a class of minerals containing sulfide or disulfide as the major anion. Sulfosalt minerals are those complex sulfide minerals with the general formula: AmBnSp; where A represents a metal such as copper, lead, silver, iron, and rarely mercury, zinc, vanadium; B usually represents semi-metal such as arsenic, antimony, bismuth, and rarely germanium, or metals like tin and rarely vanadium; and S is sulfur or rarely selenium or/and tellurium (m, n, and p are integer formula subscripts). Includes sulfides, selenides, tellurides; arsenides, antimonides, bismuthides; sulfarsenites, sulfantimonites, sulfbismuthites"@en ;
  skos:exactMatch <http://linked.data.gov.au/def/minerals/sulfides-and-sulfosalts-sulfides-selenides-tellurides-arsenides-antimonides-bismuthides-sulfarsenites-sulfantimonites-sulfbismuthites-etc> ;
  skos:inScheme ming:mineralgroupvocabulary ;
  skos:prefLabel "Mineral-Sulfide or Sulfosalt"@en ;
  skos:altLabel "Nickel-Strunz class 02"@en ;
  rdf:seeAlso "https://www.mindat.org/strunz.php?a=2"
  .
ming:halidemineral
  rdf:type owl:NamedIndividual ;
  rdf:type skos:Concept ;
  rdfs:label "Mineral-Halide"@en ;
  skos:broader mat:mineral ;
  skos:definition "Minerals with a dominant halide anion."@en ;
  skos:exactMatch <http://linked.data.gov.au/def/minerals/halides> ;
  skos:inScheme ming:mineralgroupvocabulary ;
  skos:prefLabel "Mineral-Halide"@en ;
  skos:altLabel "Nickel-Strunz class 03"@en ;
  rdf:seeAlso "https://www.mindat.org/strunz.php?a=3" 
.
ming:oxidemineral
  rdf:type owl:NamedIndividual ;
  rdf:type skos:Concept ;
  rdfs:label "Mineral-Oxide"@en ;
  skos:broader mat:mineral ;
  skos:definition "Includes class oxides, hydroxides, and arsenties. Oxides are minerals in which the oxide anion is bonded to one or more metal alloys. The hydroxide-bearing minerals are typically included in the oxide class. Arsenite minerals are very rare oxygen-bearing arsenic minerals."@en ;
  skos:exactMatch <http://linked.data.gov.au/def/minerals/oxides-hydroxides-v56-vanadates-arsenites-antimonites-bismuthites-sulfites-selenites-tellurites-iodates> ;
  skos:inScheme ming:mineralgroupvocabulary ;
  skos:prefLabel "Mineral-Oxide"@en ;
  skos:altLabel "Nickel-Strunz class 04"@en ;
  rdf:seeAlso "https://www.mindat.org/strunz.php?a=4" 
.
ming:carbonatenitratemineral
  rdf:type owl:NamedIndividual ;
  rdf:type skos:Concept ;
  rdfs:label "Mineral-Carbonate or Nitrate"@en ;
  skos:broader mat:mineral ;
  skos:definition "Carbonate minerals are those minerals containing the carbonate ion"@en ;
  skos:exactMatch <http://linked.data.gov.au/def/minerals/carbonates-nitrates> ;
  skos:inScheme ming:mineralgroupvocabulary ;
  skos:prefLabel "Mineral-Carbonate or Nitrate"@en ;
  skos:altLabel "Nickel-Strunz class 05"@en ;
  rdf:seeAlso "https://www.mindat.org/strunz.php?a=5" 
.
ming:boratemineral
  rdf:type owl:NamedIndividual ;
  rdf:type skos:Concept ;
  rdfs:label "Mineral-Borate"@en ;
  skos:broader mat:mineral ;
  skos:definition "Minerals which contain a borate anion group."@en ;
  skos:exactMatch <http://linked.data.gov.au/def/minerals/borates> ;
  skos:inScheme ming:mineralgroupvocabulary ;
  skos:prefLabel "Mineral-Borate"@en ;
  skos:altLabel "Nickel-Strunz class 06"@en ;
  rdf:seeAlso "https://www.mindat.org/strunz.php?a=6" 
.
ming:sulfateselenatetelluratemineral
  rdf:type owl:NamedIndividual ;
  rdf:type skos:Concept ;
  rdfs:label "Mineral-Sulfate, Selenate, or Tellurate"@en ;
  skos:broader mat:mineral ;
  skos:definition "class of minerals that include the sulfate ion within their structure. "@en ;
  skos:exactMatch <http://linked.data.gov.au/def/minerals/sulfates-selenates-tellurates-chromates-molybdates-wolframates> ;
  skos:inScheme ming:mineralgroupvocabulary ;
  skos:prefLabel "Mineral-Sulfate, Selenate, or Tellurate"@en ;
  skos:altLabel "Nickel-Strunz class 07"@en ;
  rdf:seeAlso "https://www.mindat.org/strunz.php?a=7" 
.
ming:phosphatearsenatevanadatemineral
  rdf:type owl:NamedIndividual ;
  rdf:type skos:Concept ;
  rdfs:label "Mineral-Phosphate, Arsenate, or Vanadate"@en ;
  skos:broader mat:mineral ;
  skos:definition "Phosphate minerals contain the phosphate anion along sometimes with arsenate and vanadate substitutions, and chloride, fluoride, and hydroxide anions that also fit into the crystal structure. Arsenate minerals usually refer to the naturally occurring orthoarsenates."@en ;
  skos:exactMatch <http://linked.data.gov.au/def/minerals/phosphates-arsenates-vanadates> ;
  skos:inScheme ming:mineralgroupvocabulary ;
  skos:prefLabel "Mineral-Phosphate, Arsenate, or Vanadate"@en ;
  skos:altLabel "Nickel-Strunz class 08"@en ;
  rdf:seeAlso "https://www.mindat.org/strunz.php?a=8" 
.
ming:silicategermanatemineral
  rdf:type owl:NamedIndividual ;
  rdf:type skos:Concept ;
  rdfs:label "Mineral-Silicate or Germanate"@en ;
  skos:broader mat:mineral ;
  skos:definition "Rock-forming minerals made up of silicate groups"@en ;
  skos:exactMatch <http://linked.data.gov.au/def/minerals/silicates-germanates> ;
  skos:inScheme ming:mineralgroupvocabulary ;
  skos:prefLabel "Mineral-Silicate or Germanate"@en ;
  skos:altLabel "Nickel-Strunz class 09"@en ;
  rdf:seeAlso "https://www.mindat.org/strunz.php?a=9" 
.